DY/EquationalTheory/Literal.lean
@@ -1,10 +1,11 @@
-import DY.Trace.Basic
-import DY.Label
-import DY.Bytes
-import DY.Misc
+module
+
+public import DY.Bytes
+public import DY.Misc.Instances
 
 namespace DY.Literal
 
+public
 class CanMkLiteral (Bytes: Type u) where
   literalToBytes: ByteArray → Bytes
   bytesToLiteral: Bytes → Option ByteArray
@@ -16,12 +17,15 @@ export CanMkLiteral (bytesToLiteral)
 
 section Constructors
 
+public
 structure Literal (Bytes: Type) where
   lit: ByteArray
 
+public
 instance: ALaCarte.FunctorSizeOf Literal where
   sizeOf | {lit := _} => 0
 
+public
 instance: ALaCarte.Representable Literal where
   CtorId := Unit
   ctors | () => { Data := ByteArray, nRec := 0 }
@@ -40,20 +44,26 @@ instance: ALaCarte.Representable Literal where
     simp_all <;> grind
   sizeOf_eq | {lit := _} => by simp +arith [ALaCarte.FunctorSizeOf.sizeOf]
 
-instance: ALaCarte.RepresentableDecidableEq Literal where
-instance: ALaCarte.RepresentableOrd Literal where
-instance: SubBytesFunctor Literal where
+public instance: ALaCarte.RepresentableDecidableEq Literal where
+public instance: ALaCarte.RepresentableOrd Literal where
 
+public instance: SubBytesFunctor Literal where
+
+public
 abbrev SubF := Literal
 
+public
 def Literal.length [BytesFunctor]: Bytes.PartialLength Literal :=
   fun { lit := lit } _ =>
     lit.size
 
+public
 abbrev SubF.length [BytesFunctor]: Bytes.PartialLength SubF := Literal.length
 
+public
 abbrev Literal.pack [BytesFunctor] [BytesFunctor.Has SubF] (x: Literal Bytes) := BytesView.pack x
 
+public
 instance [BytesFunctor] [BytesFunctor.Has SubF]: CanMkLiteral Bytes where
   literalToBytes lit :=
     ({ lit }: Literal Bytes).pack
@@ -64,6 +74,7 @@ instance [BytesFunctor] [BytesFunctor.Has SubF]: CanMkLiteral Bytes where
       some lit
     | none => none
 
+public
 theorem bytesToLiteral_literalToBytes
   [BytesFunctor] [BytesFunctor.Has SubF]
   (lit: ByteArray)
@@ -72,6 +83,7 @@ theorem bytesToLiteral_literalToBytes
   simp only [bytesToLiteral, literalToBytes]
   grind
 
+public
 theorem literalToBytes_bytesToLiteral
   [BytesFunctor] [BytesFunctor.Has SubF]
   (buf: Bytes)
@@ -89,15 +101,18 @@ section AttackerKnowledge
 
 variable [BytesFunctor] [BytesFunctor.Has SubF]
 
+public
 def attKnowsLit: SubAttackerKnowledge Literal where
   pred p out :=
     ∃ lit,
       out = literalToBytes lit
 
+public
 abbrev attackerKnowledge := attKnowsLit
 
 variable [AttackerKnowledge] [AttackerKnowledge.Has attackerKnowledge]
 
+public
 theorem attacker_knows_literalToBytes
   (lit: ByteArray) (tr: Trace α)
   : (literalToBytes lit: Bytes).AttackerKnows tr
@@ -112,6 +127,7 @@ section Invariants
 
 variable [BytesFunctor] [BytesFunctor.Has SubF]
 
+public
 def Literal.invariants: Bytes.PartialInvariants Literal where
   well_formed := fun {lit := _} _rec _tr =>
     True
@@ -124,15 +140,19 @@ def Literal.invariants: Bytes.PartialInvariants Literal where
   invariant := fun {lit := _} _rec _tr =>
     True
 
+public
 abbrev invariants: Bytes.PartialInvariants SubF := Literal.Literal.invariants
 
+public
 def Literal.invariantsProofs [BytesInvariants]: Bytes.PartialInvariantsProofs Literal.invariants where
 
+public
 abbrev invariantsProofs [BytesInvariants]: Bytes.PartialInvariantsProofs invariants := Literal.Literal.invariantsProofs
 
 variable [BytesInvariants] [BytesInvariants.Has invariants]
 
 @[simp]
+public
 theorem literalToBytes.WellFormed
   (lit: ByteArray) (tr: ProofTrace)
   : (literalToBytes lit: Bytes).WellFormed tr
@@ -140,6 +160,7 @@ theorem literalToBytes.WellFormed
   simp [literalToBytes, Bytes.WellFormed.eq, Literal.invariants]
 
 @[simp]
+public
 theorem literalToBytes.label
   (lit: ByteArray) (tr: ProofTrace)
   : (literalToBytes lit: Bytes).label tr = Label.pub
@@ -147,6 +168,7 @@ theorem literalToBytes.label
   simp [literalToBytes, Bytes.label.eq, Literal.invariants]
 
 @[simp]
+public
 theorem literalToBytes.Invariant
   (lit: ByteArray) (tr: ProofTrace)
   : (literalToBytes lit: Bytes).Invariant tr
@@ -161,6 +183,7 @@ variable [BytesFunctor] [BytesInvariants]
 variable [BytesFunctor.Has SubF]
 variable [BytesInvariants.Has invariants]
 
+public
 instance: SubAttackerKnowledgeTheorem attKnowsLit where
   pf := by
     simp only [attKnowsLit]
