DY/Label/Labels.lean
@@ -1,15 +1,19 @@
-import DY.Label.Basic
-import DY.Trace.Basic
+module
+
+public import DY.Label.Basic
+public import DY.Trace.Basic
 
 namespace DY
 
 variable [BytesFunctor]
 
+public
 structure LabelCtor where
   isCorrupt: Trace Unit → Prop
   isCorruptLater:
     ∀ tr1 tr2, tr1 ≤ tr2 ∧ isCorrupt tr1 → isCorrupt tr2
 
+public
 def Label.make (l: LabelCtor): Label := {
   isCorrupt_ := l.isCorrupt
   isCorruptSnoc_ := by
@@ -22,14 +26,17 @@ def Label.make (l: LabelCtor): Label := {
     · assumption
 }
 
+public
 def Label.isCorrupt (l: Label) (tr: Trace α) :=
   l.isCorrupt_ tr.erase
 
 @[simp, grind]
+public
 theorem Label.makeIsCorrupt (ctor: LabelCtor) (tr: Trace α): (Label.make ctor).isCorrupt tr = ctor.isCorrupt tr.erase := by
   simp [Label.make, isCorrupt]
 
 @[scoped grind→]
+public
 theorem _root_.DY.Trace.MonotoneLemmas.isCorrupt_Later (l: Label) (tr1 tr2: Trace Unit):
   tr1 ≤ tr2 →
   l.isCorrupt_ tr1 →
@@ -44,6 +51,7 @@ theorem _root_.DY.Trace.MonotoneLemmas.isCorrupt_Later (l: Label) (tr1 tr2: Trac
       grind
 
 @[scoped grind→]
+public
 theorem _root_.DY.Trace.MonotoneLemmas.isCorruptLater (l: Label) (tr1 tr2: Trace α):
   tr1 ≤ tr2 →
   l.isCorrupt tr1 →
@@ -56,6 +64,7 @@ theorem _root_.DY.Trace.MonotoneLemmas.isCorruptLater (l: Label) (tr1 tr2: Trace
     assumption
 
 @[ext]
+public
 theorem Label.ext
   (l1 l2: Label)
   : (∀ tr: Trace Unit, l1.isCorrupt tr = l2.isCorrupt tr) →
@@ -69,12 +78,15 @@ theorem Label.ext
     have := Trace.erase_idempotent tr
     grind
 
+@[expose]
+public
 def Label.canFlow (l1: Label) (l2: Label) (tr: Trace α): Prop :=
   ∀ trLater,
     tr ≤ trLater →
     l2.isCorrupt trLater → l1.isCorrupt trLater
 
 @[scoped grind→]
+public
 theorem _root_.DY.Trace.MonotoneLemmas.canFlowLater (l1: Label) (l2: Label) (tr1 tr2: Trace α):
   tr1 ≤ tr2 →
   l1.canFlow l2 tr1 →
@@ -84,6 +96,7 @@ theorem _root_.DY.Trace.MonotoneLemmas.canFlowLater (l1: Label) (l2: Label) (tr1
     grind [Trace.trace_le_trans]
 
 @[grind]
+public
 theorem canFlowRefl (l: Label) (tr: Trace α):
   l.canFlow l tr
   := by
@@ -91,6 +104,7 @@ theorem canFlowRefl (l: Label) (tr: Trace α):
     grind
 
 -- @[grind]
+public
 theorem canFlowTrans (l1: Label) (l2: Label) (l3: Label) (tr: Trace α):
   l1.canFlow l2 tr →
   l2.canFlow l3 tr →
@@ -99,16 +113,19 @@ theorem canFlowTrans (l1: Label) (l2: Label) (l3: Label) (tr: Trace α):
     unfold Label.canFlow
     grind
 
+public
 def Label.pub : Label := Label.make {
   isCorrupt tr := True
   isCorruptLater := by grind
 }
 
 @[simp, grind]
+public
 theorem Label.pubIsCorrupt (tr: Trace α): Label.pub.isCorrupt tr := by
   grind [Label.pub]
 
 @[grind =_]
+public
 theorem canFlowPubEqIsCorrupt (l: Label) (tr: Trace α):
   l.isCorrupt tr = l.canFlow Label.pub tr
   := by
@@ -116,50 +133,59 @@ theorem canFlowPubEqIsCorrupt (l: Label) (tr: Trace α):
   -- open DY.Trace.MonotoneLemmas in
   grind [Label.canFlow, DY.Trace.MonotoneLemmas.isCorruptLater]
 
+public
 def Label.secret : Label := Label.make {
   isCorrupt tr := False
   isCorruptLater := by grind
 }
 
 @[simp, grind]
+public
 theorem Label.secretIsCorrupt (tr: Trace α): ¬ Label.secret.isCorrupt tr := by
   grind [secret]
 
 @[grind]
+public
 theorem Label.secret.canFlow (l: Label) (tr: Trace α):
   l.canFlow secret tr
   := by
   grind [Label.canFlow]
 
+public
 def Label.join (l1 l2: Label): Label := Label.make {
   isCorrupt tr := l1.isCorrupt_ tr ∨ l2.isCorrupt_ tr
   isCorruptLater := by grind
 }
 
 @[simp, grind]
+public
 theorem Label.joinIsCorrupt (l1 l2: Label) (tr: Trace α):
   (l1.join l2).isCorrupt tr = (l1.isCorrupt tr ∨ l2.isCorrupt tr)
   := by
   grind [join, isCorrupt]
 
+public
 def Label.meet (l1 l2: Label): Label := Label.make {
   isCorrupt tr := l1.isCorrupt_ tr ∧ l2.isCorrupt_ tr
   isCorruptLater := by grind
 }
 
 @[simp, grind]
+public
 theorem Label.meetIsCorrupt (l1 l2: Label) (tr: Trace α):
   (l1.meet l2).isCorrupt tr = (l1.isCorrupt tr ∧ l2.isCorrupt tr)
   := by
   grind [meet, isCorrupt]
 
 @[grind =]
+public
 theorem Label.joinEq (l1: Label) (l2: Label) (l3: Label) (tr: Trace α):
   l1.canFlow (l2.join l3) tr = (l1.canFlow l2 tr ∧ l1.canFlow l3 tr)
   := by
   grind [canFlow]
 
 @[grind]
+public
 theorem Label.joinCanFlowLeft (l1: Label) (l2: Label) (tr: Trace α):
   (l1.join l2).canFlow l1 tr
   := by
@@ -167,6 +193,7 @@ theorem Label.joinCanFlowLeft (l1: Label) (l2: Label) (tr: Trace α):
   grind
 
 @[grind]
+public
 theorem Label.joinCanFlowRight (l1: Label) (l2: Label) (tr: Trace α):
   (l1.join l2).canFlow l2 tr
   := by
@@ -174,15 +201,18 @@ theorem Label.joinCanFlowRight (l1: Label) (l2: Label) (tr: Trace α):
   grind
 
 @[grind]
+public
 theorem Label.join_pub_left (l: Label): Label.join Label.pub l = Label.pub := by
   ext
   grind
 
 @[grind]
+public
 theorem Label.join_pub_right (l: Label): Label.join l Label.pub = Label.pub := by
   ext
   grind
 
+public
 theorem Label.join_commutes (l1 l2: Label): Label.join l1 l2 = Label.join l2 l1 := by
   ext
   grind
