DY/Misc/Instances.lean
@@ -1,29 +1,40 @@
+module
+
+public
 instance: Ord Unit where
   compare _ _ := .eq
 
+public
 instance: Std.ReflOrd Unit where
   compare_self := by grind
 
+public
 instance: Std.LawfulEqOrd Unit where
   eq_of_compare := by grind
 
+public
 instance: Std.OrientedOrd Unit where
   eq_swap := by grind [Ordering.swap]
 
+public
 instance: Std.TransOrd Unit where
   isLE_trans := by grind
 
+public
 def ByteArray.compare (x y: ByteArray): Ordering :=
   Ord.compare x.data y.data
 
+public
 instance: Ord ByteArray where
   compare x y := ByteArray.compare x y
 
+public
 instance: Std.ReflOrd ByteArray where
   compare_self := by
     simp only [compare]
     simp [ByteArray.compare]
 
+public
 instance: Std.LawfulEqOrd ByteArray where
   eq_of_compare := by
     simp only [compare]
@@ -33,6 +44,7 @@ instance: Std.LawfulEqOrd ByteArray where
     apply Std.LawfulEqOrd.eq_of_compare
     exact h
 
+public
 instance: Std.OrientedOrd ByteArray where
   eq_swap := by
     simp only [compare]
@@ -40,6 +52,7 @@ instance: Std.OrientedOrd ByteArray where
     intro x y
     apply Std.OrientedOrd.eq_swap
 
+public
 instance: Std.TransOrd ByteArray where
   isLE_trans := by
     simp only [compare]
