DY/Trace.lean
@@ -1,2 +1,4 @@
-import DY.Trace.Basic
-import DY.Trace.Manipulation
+module
+
+public import DY.Trace.Basic
+public import DY.Trace.Manipulation
